LambdaS5/coq/LjsPrettyRulesAux.v
@@ -34,35 +34,70 @@ Proof.
     inverts Hred; tryfalse; injects; jauto.
 Qed.
 
-Fixpoint pure_expr_pred c st e v : Prop :=
+Require Import LibEpsilon. (* TODO move *)
+
+Instance attributes_inhab : Inhab attributes.
+Proof. intros. apply (prove_Inhab (attributes_data_of (attributes_data_intro value_null false false false))). Qed.
+
+Instance object_inhab : Inhab object.
+Proof. intros. apply (prove_Inhab default_object). Qed.
+
+Fixpoint pure_expr_val c st e : value :=
     match e with
-    | expr_undefined => v = value_undefined
-    | expr_null => v = value_null
-    | expr_empty => v = value_empty
-    | expr_bool b => v = value_bool b
-    | expr_string s => v = value_string s
-    | expr_number n => v = value_number n
-    | expr_lambda is e => v = add_closure c None is e
-    | expr_id s => binds c s v 
-    | expr_if e1 e2 e3 => exists b, pure_expr_pred c st e1 (value_bool b) /\ 
-        (b /\ pure_expr_pred c st e2 v \/ ~b /\ pure_expr_pred c st e3 v) 
-    | expr_let s e1 e2 => exists v', pure_expr_pred c st e1 v' /\ pure_expr_pred (c \(s := v')) st e2 v
-    | expr_seq e1 e2 => pure_expr_pred c st e2 v
-    | expr_jseq e1 e2 => exists v1 v2, pure_expr_pred c st e1 v1 /\ pure_expr_pred c st e2 v2 /\
-        v = overwrite_value_if_empty v1 v2
-    | expr_op1 op e => exists v', pure_expr_pred c st e v' /\ eval_unary_op op st v' v
-    | expr_op2 op e1 e2 => exists v1 v2, pure_expr_pred c st e1 v1 /\ pure_expr_pred c st e2 v2 /\
-        eval_binary_op op st v1 v2 v
-    | expr_get_attr pa e1 e2 => exists ptr obj s attrs, 
-        pure_expr_pred c st e1 (value_object ptr) /\ 
-        pure_expr_pred c st e2 (value_string s) /\
-        binds st ptr obj /\ binds (object_properties obj) s attrs /\
-        attributes_pattr_readable attrs pa /\ v = get_attributes_pattr attrs pa
-    | expr_get_obj_attr oa e => exists ptr obj,
-        pure_expr_pred c st e (value_object ptr) /\
-        binds st ptr obj /\
-        v = get_object_oattr obj oa
-    | _ => False
+    | expr_undefined => value_undefined
+    | expr_null => value_null
+    | expr_empty => value_empty
+    | expr_bool b => value_bool b
+    | expr_string s => value_string s
+    | expr_number n => value_number n
+    | expr_lambda is e => add_closure c None is e
+    | expr_id s => epsilon (binds c s) 
+    | expr_if e1 e2 e3 => 
+        match pure_expr_val c st e1 with
+        | value_bool true => pure_expr_val c st e2
+        | value_bool false => pure_expr_val c st e3
+        | _ => arbitrary
+        end
+    | expr_let s e1 e2 => pure_expr_val (c \(s := pure_expr_val c st e1)) st e2
+    | expr_seq e1 e2 => pure_expr_val c st e2
+    | expr_jseq e1 e2 => overwrite_value_if_empty (pure_expr_val c st e1) (pure_expr_val c st e2)
+    | expr_op1 op e => epsilon (eval_unary_op op st (pure_expr_val c st e))
+    | expr_op2 op e1 e2 => epsilon (eval_binary_op op st (pure_expr_val c st e1) (pure_expr_val c st e2))
+    | expr_get_attr pa e1 e2 => 
+        match pure_expr_val c st e1, pure_expr_val c st e2 with
+        | value_object ptr, value_string s => 
+            get_attributes_pattr (epsilon (binds (object_properties (epsilon (binds st ptr))) s)) pa
+        | _, _ => arbitrary
+        end
+    | expr_get_obj_attr oa e =>
+        match pure_expr_val c st e with
+        | value_object ptr => get_object_oattr (epsilon (binds st ptr)) oa
+        | _ => arbitrary
+        end
+    | _ => value_undefined
+    end.
+
+Fixpoint pure_expr_pre c st e : Prop :=
+    match e with
+    | expr_id s => exists v, binds c s v
+    | expr_if e1 e2 e3 => pure_expr_pre c st e1 /\
+        (exists b, pure_expr_val c st e1 = value_bool b /\ 
+            (b -> pure_expr_pre c st e2) /\ (~b -> pure_expr_pre c st e3))
+    | expr_let s e1 e2 => pure_expr_pre c st e1 /\ pure_expr_pre (c\(s := pure_expr_val c st e1)) st e2
+    | expr_seq e1 e2 => pure_expr_pre c st e1 /\ pure_expr_pre c st e2
+    | expr_jseq e1 e2 => pure_expr_pre c st e1 /\ pure_expr_pre c st e2
+    | expr_op1 op e => pure_expr_pre c st e /\ 
+        exists v, eval_unary_op op st (pure_expr_val c st e) v
+    | expr_op2 op e1 e2 => pure_expr_pre c st e1 /\ pure_expr_pre c st e2 /\
+        exists v, eval_binary_op op st (pure_expr_val c st e1) (pure_expr_val c st e2) v
+    | expr_get_attr pa e1 e2 => pure_expr_pre c st e1 /\ pure_expr_pre c st e2 /\
+        (exists ptr obj s attrs, 
+            pure_expr_val c st e1 = value_object ptr /\ pure_expr_val c st e2 = value_string s /\
+            binds st ptr obj /\ binds (object_properties obj) s attrs /\
+            attributes_pattr_readable attrs pa)
+    | expr_get_obj_attr oa e => pure_expr_pre c st e /\
+        (exists ptr obj, pure_expr_val c st e = value_object ptr /\ binds st ptr obj)
+    | _ => True
     end.
 
 Fixpoint bool_expr_pred c st e : Prop :=
@@ -72,97 +107,130 @@ Fixpoint bool_expr_pred c st e : Prop :=
     | expr_if e1 e2 e3 => 
         bool_expr_pred c st e1 /\ bool_expr_pred c st e2 \/ ~bool_expr_pred c st e1 /\ bool_expr_pred c st e3
     | expr_let s e1 e2 =>
-        exists v, pure_expr_pred c st e1 v /\ bool_expr_pred (c \(s := v)) st e2
-    | expr_op1 unary_op_is_primitive e => exists v, pure_expr_pred c st e v /\ is_primitive v
-    | expr_op1 unary_op_is_closure e => exists v, pure_expr_pred c st e v /\ is_closure v
-    | expr_op1 unary_op_is_object e => exists v, pure_expr_pred c st e v /\ is_object v
-    | expr_op1 unary_op_prim_to_bool e => exists v, pure_expr_pred c st e v /\ value_to_bool_cast v
+        bool_expr_pred (c \(s := pure_expr_val c st e1)) st e2
+    | expr_op1 unary_op_is_primitive e => is_primitive (pure_expr_val c st e)
+    | expr_op1 unary_op_is_closure e => is_closure (pure_expr_val c st e)
+    | expr_op1 unary_op_is_object e => is_object (pure_expr_val c st e)
+    | expr_op1 unary_op_prim_to_bool e => value_to_bool_cast (pure_expr_val c st e)
     | expr_op1 unary_op_not e => ~bool_expr_pred c st e
     | expr_op2 binary_op_stx_eq e1 e2 => 
-        exists v1 v2, pure_expr_pred c st e1 v1 /\ pure_expr_pred c st e2 v2 /\ stx_eq v1 v2
+        stx_eq (pure_expr_val c st e1) (pure_expr_val c st e2)
     | expr_op2 binary_op_same_value e1 e2 => 
-        exists v1 v2, pure_expr_pred c st e1 v1 /\ pure_expr_pred c st e2 v2 /\ same_value v1 v2
+        same_value (pure_expr_val c st e1) (pure_expr_val c st e2)
     | expr_op2 binary_op_has_property e1 e2 => 
-        exists ptr obj s, pure_expr_pred c st e1 (value_object ptr) /\ pure_expr_pred c st e2 (value_string s) /\
-        binds st ptr obj /\ exists att, object_property_is st obj s (Some att)
+        match pure_expr_val c st e1, pure_expr_val c st e2 with
+        | value_object ptr, value_string s =>
+            is_some (epsilon (object_property_is st (epsilon (binds st ptr)) s))
+        | _, _ => False
+        end
     | expr_op2 binary_op_has_own_property e1 e2 => 
-        exists ptr obj s, pure_expr_pred c st e1 (value_object ptr) /\ pure_expr_pred c st e2 (value_string s) /\
-        binds st ptr obj /\ index (object_properties obj) s
+        match pure_expr_val c st e1, pure_expr_val c st e2 with
+        | value_object ptr, value_string s =>
+            index (object_properties (epsilon (binds st ptr))) s
+        | _, _ => False
+        end
     | expr_op2 binary_op_has_internal e1 e2 => 
-        exists ptr obj s, pure_expr_pred c st e1 (value_object ptr) /\ pure_expr_pred c st e2 (value_string s) /\
-        binds st ptr obj /\ index (object_internal obj) s
+        match pure_expr_val c st e1, pure_expr_val c st e2 with
+        | value_object ptr, value_string s =>
+            index (object_internal (epsilon (binds st ptr))) s
+        | _, _ => False
+        end
     | expr_op2 binary_op_is_accessor e1 e2 => 
-        exists ptr obj s att, pure_expr_pred c st e1 (value_object ptr) /\ pure_expr_pred c st e2 (value_string s) /\
-        binds st ptr obj /\ object_property_is st obj s (Some att) /\ is_accessor att
+        match pure_expr_val c st e1, pure_expr_val c st e2 with
+        | value_object ptr, value_string s =>
+            is_accessor (unsome (epsilon (object_property_is st (epsilon (binds st ptr)) s)))
+        | _, _ => False
+        end
     | expr_op2 binary_op_string_lt e1 e2 => 
-        exists s1 s2, pure_expr_pred c st e1 (value_string s1) /\ pure_expr_pred c st e2 (value_string s2) /\
-        string_lt s1 s2
+        match pure_expr_val c st e1, pure_expr_val c st e2 with
+        | value_string s1, value_string s2 => string_lt s1 s2
+        | _, _ => False
+        end
     | expr_op2 binary_op_locale_compare e1 e2 => 
-        exists s1 s2, pure_expr_pred c st e1 (value_string s1) /\ pure_expr_pred c st e2 (value_string s2) /\
-        string_lt s1 s2
+        match pure_expr_val c st e1, pure_expr_val c st e2 with
+        | value_string s1, value_string s2 => string_lt s1 s2
+        | _, _ => False
+        end
     | expr_op2 binary_op_lt e1 e2 => 
-        exists n1 n2, pure_expr_pred c st e1 (value_number n1) /\ pure_expr_pred c st e2 (value_number n2) /\
-        num_lt n1 n2
+        match pure_expr_val c st e1, pure_expr_val c st e2 with
+        | value_number n1, value_number n2 => num_lt n1 n2
+        | _, _ => False
+        end
     | expr_op2 binary_op_gt e1 e2 => 
-        exists n1 n2, pure_expr_pred c st e1 (value_number n1) /\ pure_expr_pred c st e2 (value_number n2) /\
-        num_gt n1 n2
+        match pure_expr_val c st e1, pure_expr_val c st e2 with
+        | value_number n1, value_number n2 => num_gt n1 n2
+        | _, _ => False
+        end
     | expr_op2 binary_op_le e1 e2 => 
-        exists n1 n2, pure_expr_pred c st e1 (value_number n1) /\ pure_expr_pred c st e2 (value_number n2) /\
-        num_le n1 n2
+        match pure_expr_val c st e1, pure_expr_val c st e2 with
+        | value_number n1, value_number n2 => num_le n1 n2
+        | _, _ => False
+        end
     | expr_op2 binary_op_ge e1 e2 => 
-        exists n1 n2, pure_expr_pred c st e1 (value_number n1) /\ pure_expr_pred c st e2 (value_number n2) /\
-        num_ge n1 n2
+        match pure_expr_val c st e1, pure_expr_val c st e2 with
+        | value_number n1, value_number n2 => num_ge n1 n2
+        | _, _ => False
+        end
     | _ => False
     end.
 
-Lemma object_property_is_deterministic : forall st obj name oattr oattr',
-    object_property_is st obj name oattr -> object_property_is st obj name oattr' -> oattr = oattr'.
+Fixpoint bool_expr_pre c st e : Prop :=
+    match e with
+    | expr_bool _ => True
+    | expr_id s => exists v, binds c s v
+    | expr_if e1 e2 e3 => bool_expr_pre c st e1 /\
+        (bool_expr_pred c st e1 -> bool_expr_pre c st e2) /\ (~bool_expr_pred c st e1 -> bool_expr_pre c st e3)
+    | expr_let s e1 e2 => pure_expr_pre c st e1 /\ bool_expr_pre (c\(s := pure_expr_val c st e1)) st e2
+    | expr_op1 unary_op_not e => bool_expr_pre c st e
+    | expr_op1 op e => pure_expr_pre c st e /\
+        exists v, eval_unary_op op st (pure_expr_val c st e) v
+    | expr_op2 op e1 e2 => pure_expr_pre c st e1 /\ pure_expr_pre c st e2 /\
+        exists v, eval_binary_op op st (pure_expr_val c st e1) (pure_expr_val c st e2) v
+    | _ => False
+    end.
+
+Instance object_property_is_deterministic : forall st obj name, Deterministic (object_property_is st obj name).
 Proof.
+    introv. constructor.
     introv Ho1.
     induction Ho1; introv Ho2; inverts Ho2; 
-    repeat binds_determine; substs; tryfalse; try reflexivity; try (false; prove_bag). 
-    rewrite H0 in H6.
-    injects.
-    binds_determine; substs.
+    repeat determine; substs; tryfalse; try reflexivity; try (false; prove_bag).
     auto.
 Qed.
 
-Lemma value_is_closure_deterministic : forall st v clo clo',
-    value_is_closure st v clo -> value_is_closure st v clo' -> clo = clo'.
+Instance value_is_closure_deterministic : forall st v, Deterministic (value_is_closure st v).
 Proof.
+    introv. constructor.
     introv Hc1.
     induction Hc1; introv Hc2; inverts Hc2.
     reflexivity.
-    binds_determine.
-    substs.
+    determine.
     auto.
 Qed.
 
-Lemma closure_ctx_deterministic : forall clo lv c c',
-    closure_ctx clo lv c -> closure_ctx clo lv c' -> c = c'.
+Instance closure_ctx_deterministic : forall clo lv, Deterministic (closure_ctx clo lv).
 Proof.
+    introv. constructor.
     introv Hc1.
     induction Hc1; introv Hc2; inverts Hc2;
     repeat match goal with H : Zip _ _ _ |- _ => apply Zip_zip in H end;
     rewrite H in *; injects; reflexivity.
 Qed.
 
-Lemma eval_unary_op_deterministic : forall op st v0 v v',
-    eval_unary_op op st v0 v -> eval_unary_op op st v0 v' -> v = v'.
+Instance eval_unary_op_deterministic : forall op st v0, Deterministic (eval_unary_op op st v0).
 Proof.
+    introv. constructor.
     introv He1 He2.
     destruct op; inverts He1 as Hu1; try inverts Hu1; inverts He2 as Hu2; try inverts Hu2;
     reflexivity.
 Qed.
 
-Lemma eval_binary_op_deterministic : forall op st v1 v2 v v',
-    eval_binary_op op st v1 v2 v -> eval_binary_op op st v1 v2 v' -> v = v'.
+Instance eval_binary_op_deterministic : forall op st v1 v2, Deterministic (eval_binary_op op st v1 v2).
 Proof.
+    introv. constructor.
     introv He1 He2.
     destruct op; inverts He1 as Hu1; try inverts Hu1; inverts He2 as Hu2; try inverts Hu2;
-    repeat binds_determine; try reflexivity.
-    rewrite H1 in *. injects. reflexivity. 
-    lets X : object_property_is_deterministic H1 H5. injects. reflexivity.
+    repeat determine; try reflexivity.
 Qed.
 
 Ltac false_abort := 
@@ -173,20 +241,23 @@ Ltac false_abort :=
 Lemma pure_expr_lemma : forall c st st' e r,
     pure_expr e ->
     red_expr c st e (out_ter st' r) ->
-    st = st' /\ exists v,
-    r = res_value v /\ pure_expr_pred c st e v.
+    st = st' /\ pure_expr_pre c st e /\
+    r = res_value (pure_expr_val c st e).
 Proof.
     introv Hpe Hred.
     inductions Hpe gen c st st' r Hred;
     inverts Hred as Hr1 Hr2; simpl; jauto.
+    (* id *)
+    determine_epsilon.
+    jauto.
     (* if *)
     forwards Hx : out_red_ter Hr2. reflexivity. destruct_hyp Hx.
     specializes IHHpe1 Hr1. destruct_hyp IHHpe1.
     inverts Hr2 as Hr2.
-    specializes IHHpe2 Hr2. destruct_hyp IHHpe2.
-    jauto.
-    specializes IHHpe3 Hr2. destruct_hyp IHHpe3.
-    jauto.
+    specializes IHHpe2 Hr2. destruct_hyp IHHpe2. simpl. 
+    jauto_set; eauto. rew_refl. iauto.
+    specializes IHHpe3 Hr2. destruct_hyp IHHpe3. simpl. 
+    jauto_set; eauto. rew_refl. iauto.
     false_abort.
     (* seq *)
     forwards Hx : out_red_ter Hr2. reflexivity. destruct_hyp Hx.
@@ -214,7 +285,7 @@ Proof.
     forwards Hx : out_red_ter Hr2. reflexivity. destruct_hyp Hx.
     specializes IHHpe Hr1. destruct_hyp IHHpe.
     inverts Hr2 as Hr2; [idtac | false_abort].
-    jauto.
+    determine_epsilon. jauto.
     (* binary *)    
     forwards Hx : out_red_ter Hr2. reflexivity. destruct_hyp Hx.
     specializes IHHpe1 Hr1. destruct_hyp IHHpe1.
@@ -222,7 +293,7 @@ Proof.
     forwards Hx : out_red_ter Hr3. reflexivity. destruct_hyp Hx.
     specializes IHHpe2 Hr2. destruct_hyp IHHpe2.
     inverts Hr3 as Hr3; [idtac | false_abort].
-    jauto.
+    determine_epsilon. jauto.
     (* get_attr *)
     inverts Hr1 as Hr1 Hr2.
     forwards Hx : out_red_ter Hr2. reflexivity. destruct_hyp Hx.
@@ -233,166 +304,57 @@ Proof.
     specializes IHHpe2 Hr2. destruct_hyp IHHpe2.
     inverts Hr3 as Hr3; [idtac | false_abort].
     inverts Hr3 as Hr3. inverts Hr3 as Hr3.
-    jauto.
+    do 2 determine_epsilon. jauto.
     (* get_obj_attr *)
     forwards Hx : out_red_ter Hr2. reflexivity. destruct_hyp Hx.
     specializes IHHpe Hr1. destruct_hyp IHHpe.
     inverts Hr2 as Hr2; [idtac | false_abort].
-    jauto.
+    determine_epsilon. jauto.
 Qed.
 
-Lemma pure_expr_pred_deterministic : forall c st e v v',
-    pure_expr_pred c st e v -> pure_expr_pred c st e v' -> v = v'.
+Local Hint Constructors red_expr.
+
+Lemma pure_expr_lemma_inv : forall c st e,
+    pure_expr e -> pure_expr_pre c st e -> red_expr c st e (out_ter st (res_value (pure_expr_val c st e))).
 Proof.
-    introv Hpe1 Hpe2.
-    inductions e gen c st Hpe1 Hpe2; simpls; substs; repeat binds_determine; try reflexivity; tryfalse.
-    (* get_attr *)
-    destruct Hpe1 as (?ptr&?obj&?s&?attrs&Hpe1&Hpf1&Hb1&Hbp1&Hre1&Heq1).
-    destruct Hpe2 as (?ptr&?obj&?s&?attrs&Hpe2&Hpf2&Hb2&Hbp2&Hre2&Heq2).
-    specializes IHe1 Hpe1 Hpe2.
-    specializes IHe2 Hpf1 Hpf2.
-    repeat injects. substs. repeat binds_determine.
-    reflexivity.
-    (* get_obj_attr *)
-    destruct Hpe1 as (?ptr&?obj&Hpe1&Hb1&Heq1).
-    destruct Hpe2 as (?ptr&?obj&Hpe2&Hb2&Heq2).
-    specializes IHe Hpe1 Hpe2.
-    repeat injects. substs. repeat binds_determine.
-    reflexivity.
-    (* unary *)
-    destruct Hpe1 as (?v&Hpe1&Hun1).
-    destruct Hpe2 as (?v&Hpe2&Hun2).
-    specializes IHe Hpe1 Hpe2. substs.
-    applys eval_unary_op_deterministic Hun1 Hun2.
-    (* binary *)
-    destruct Hpe1 as (?v&?v&Hpe1&Hpf1&Hun1).
-    destruct Hpe2 as (?v&?v&Hpe2&Hpf2&Hun2).
-    specializes IHe1 Hpe1 Hpe2.
-    specializes IHe2 Hpf1 Hpf2. substs.
-    applys eval_binary_op_deterministic Hun1 Hun2.
+    introv Hpe Hpre.
+    inductions Hpe gen c st Hpre; simpls; jauto.
+    (* id *)
+    destruct_hyp Hpre.
+    determine_epsilon. eauto.
     (* if *)
-    destruct Hpe1 as (b1&Hpe1&Hcond1).
-    destruct Hpe2 as (b2&Hpe2&Hcond2).
-    specializes IHe1 Hpe1 Hpe2.
-    injects.
-    destruct b2;
-    rew_refl in Hcond1; rew_refl in Hcond2;
-    rew_logic in Hcond1; rew_logic in Hcond2.
-    specializes IHe2 Hcond1 Hcond2.
-    specializes IHe3 Hcond1 Hcond2.
-    (* seq *)
-    eauto.
-    (* jseq *)
-    destruct Hpe1 as (?v&?v&Hpe1&Hpf1&Heq1).
-    destruct Hpe2 as (?v&?v&Hpe2&Hpf2&Heq2).
-    specializes IHe1 Hpe1 Hpe2.
-    specializes IHe2 Hpf1 Hpf2.
-    substs. reflexivity.
-    (* let *)
-    destruct Hpe1 as (?v&Hpe1&Hpf1).
-    destruct Hpe2 as (?v&Hpe2&Hpf2).
-    specializes IHe1 Hpe1 Hpe2. substs.
-    specializes IHe2 Hpf1 Hpf2.
+    destruct_hyp Hpre.
+    specializes IHHpe1 ___. eassumption.
+    rewrite Hpre2 in *. (* TODO *)
+    destruct b; rew_refl in *; eauto.
+    (* op1 *)
+    destruct_hyp Hpre.
+    determine_epsilon. eauto.
+    (* op2 *)
+    destruct_hyp Hpre.
+    determine_epsilon. eauto 7.
+    (* get_attr *)
+    destruct_hyp Hpre.
+    specializes IHHpe1 ___. eassumption.
+    specializes IHHpe2 ___. eassumption.
+    rewrite Hpre1, Hpre3 in *. (* TODO *)
+    do 2 determine_epsilon. 
+    skip. (* TODO rev in eval_many *)
+    (* get_obj_attr *)
+    destruct_hyp Hpre.
+    specializes IHHpe ___. eassumption.
+    rewrite Hpre2 in *. (* TODO *)
+    determine_epsilon. eauto.
 Qed.
 
-Lemma pure_expr_pred_op1_lemma : forall P c st e v,
-    pure_expr_pred c st e v ->
-    P v = exists v', pure_expr_pred c st e v' /\ P v'.
-Proof.
-    introv Hpur.
-    rew_logic. split. jauto.
-    introv (v'&Hpur'&Hp').
-    lets Heq : pure_expr_pred_deterministic Hpur Hpur'. substs. 
-    assumption.
-Qed.
-
-Lemma pure_expr_pred_op2_lemma : forall P c st e1 e2 v1 v2,
-    pure_expr_pred c st e1 v1 ->
-    pure_expr_pred c st e2 v2 ->
-    P v1 v2 = exists v1' v2', pure_expr_pred c st e1 v1' /\ pure_expr_pred c st e2 v2' /\ P v1' v2'.
-Proof.
-    introv Hpur1 Hpur2.
-    rew_logic. split. jauto.
-    introv (v1'&v2'&Hpur1'&Hpur2'&Hp').
-    lets Heq1 : pure_expr_pred_deterministic Hpur1 Hpur1'. 
-    lets Heq2 : pure_expr_pred_deterministic Hpur2 Hpur2'. 
-    substs. 
-    assumption.
-Qed.
-
-Lemma pure_expr_pred_op2_number_lemma : forall P c st e1 e2 n1 n2,
-    pure_expr_pred c st e1 (value_number n1) ->
-    pure_expr_pred c st e2 (value_number n2) ->
-    P n1 n2 = exists n1' n2', 
-        pure_expr_pred c st e1 (value_number n1') /\ pure_expr_pred c st e2 (value_number n2') /\ P n1' n2'.
-Proof.
-    introv Hpur1 Hpur2.
-    rew_logic. split. jauto.
-    introv (v1'&v2'&Hpur1'&Hpur2'&Hp').
-    lets Heq1 : pure_expr_pred_deterministic Hpur1 Hpur1'. 
-    lets Heq2 : pure_expr_pred_deterministic Hpur2 Hpur2'. 
-    repeat injects. 
-    assumption.
-Qed.
-
-Lemma pure_expr_pred_op2_string_lemma : forall P c st e1 e2 s1 s2,
-    pure_expr_pred c st e1 (value_string s1) ->
-    pure_expr_pred c st e2 (value_string s2) ->
-    P s1 s2 = exists s1' s2', 
-        pure_expr_pred c st e1 (value_string s1') /\ pure_expr_pred c st e2 (value_string s2') /\ P s1' s2'.
-Proof.
-    introv Hpur1 Hpur2.
-    rew_logic. split. jauto.
-    introv (v1'&v2'&Hpur1'&Hpur2'&Hp').
-    lets Heq1 : pure_expr_pred_deterministic Hpur1 Hpur1'. 
-    lets Heq2 : pure_expr_pred_deterministic Hpur2 Hpur2'. 
-    repeat injects. 
-    assumption.
-Qed.
-
-Lemma pure_expr_pred_op2_object_string_lemma : forall P c st e1 e2 obj ptr s,
-    pure_expr_pred c st e1 (value_object ptr) ->
-    pure_expr_pred c st e2 (value_string s) ->
-    binds st ptr obj ->
-    P obj s = exists ptr' obj' s', 
-        pure_expr_pred c st e1 (value_object ptr') /\ pure_expr_pred c st e2 (value_string s') /\ 
-        binds st ptr' obj' /\ P obj' s'.
-Proof.
-    introv Hpur1 Hpur2 Hbinds.
-    rew_logic. split. jauto.
-    introv (obj'&ptr'&s'&Hpur1'&Hpur2'&Hbinds'&Hp').
-    lets Heq1 : pure_expr_pred_deterministic Hpur1 Hpur1'. 
-    lets Heq2 : pure_expr_pred_deterministic Hpur2 Hpur2'. 
-    repeat injects. 
-    binds_determine.
-    assumption.
-Qed.
-
-Lemma pure_expr_pred_op2_object_attrs_string_lemma : forall P c st e1 e2 obj ptr att s,
-    pure_expr_pred c st e1 (value_object ptr) ->
-    pure_expr_pred c st e2 (value_string s) ->
-    binds st ptr obj ->
-    object_property_is st obj s (Some att) ->
-    P obj s att = exists ptr' obj' s' att', 
-        pure_expr_pred c st e1 (value_object ptr') /\ pure_expr_pred c st e2 (value_string s') /\ 
-        binds st ptr' obj' /\ object_property_is st obj' s' (Some att') /\ P obj' s' att'.
-Proof.
-    introv Hpur1 Hpur2 Hbinds Hprop.
-    rew_logic. split. jauto.
-    introv (obj'&ptr'&s'&att'&Hpur1'&Hpur2'&Hbinds'&Hprop'&Hp').
-    lets Heq1 : pure_expr_pred_deterministic Hpur1 Hpur1'. 
-    lets Heq2 : pure_expr_pred_deterministic Hpur2 Hpur2'. 
-    repeat injects. 
-    binds_determine.
-    lets Heq3 : object_property_is_deterministic Hprop Hprop'.
-    injects.
-    assumption.
-Qed.
+Local Hint Constructors binary_op_type.
+Local Hint Constructors eval_unary_op.
+Local Hint Constructors eval_binary_op.
 
 Lemma bool_red_expr_lemma : forall c st st' e r,
     bool_expr e ->
-    red_expr c st e (out_ter st' r) ->
-    st = st' /\ r = res_value (value_bool (isTrue (bool_expr_pred c st e))).
+    red_expr c st e (out_ter st' r) -> 
+    st = st' /\ bool_expr_pre c st e /\ r = res_value (value_bool (isTrue (bool_expr_pred c st e))).
 Proof.
     introv Hpe Hred.
     inductions Hpe gen c st st' r Hred;
@@ -406,15 +368,13 @@ Proof.
     cases_isTrue in * as Eq;
     rew_bool;
     (inverts Hr2 as Hr2; [idtac | false_abort]). 
-    specializes IHHpe2 Hr2. destruct_hyp IHHpe2. jauto.
-    specializes IHHpe3 Hr2. destruct_hyp IHHpe3. jauto.
+    specializes IHHpe2 Hr2. destruct_hyp IHHpe2. iauto.
+    specializes IHHpe3 Hr2. destruct_hyp IHHpe3. iauto.
     (* let *)
     forwards Hx : out_red_ter Hr2. reflexivity. destruct_hyp Hx.
     forwards Hpur : pure_expr_lemma Hr1. assumption. destruct_hyp Hpur.
     inverts Hr2 as Hr2; [idtac | false_abort].
-    specializes IHHpe Hr2. destruct_hyp IHHpe. 
-    forwards Heq : pure_expr_pred_op1_lemma (fun v => bool_expr_pred (c\(s:=v)) st' e2). eassumption.
-    rewrite Heq. jauto. 
+    specializes IHHpe Hr2. destruct_hyp IHHpe. jauto. 
     (* not *)
     forwards Hx : out_red_ter Hr2. reflexivity. destruct_hyp Hx.
     specializes IHHpe Hr1. destruct_hyp IHHpe.
@@ -424,20 +384,15 @@ Proof.
     forwards Hx : out_red_ter Hr2. reflexivity. destruct_hyp Hx.
     forwards Hpur : pure_expr_lemma Hr1. assumption. destruct_hyp Hpur. clear Hr1.
     inverts Hr2 as Hr2; [idtac | false_abort].
-    destruct op; tryfalse; inverts Hr2; try false_invert.
+    destruct op; tryfalse; inverts keep Hr2; try false_invert.
     (* is_primitive *)
-    forwards Heq : pure_expr_pred_op1_lemma is_primitive. eassumption. 
-    rewrite decide_spec. rewrite Heq. jauto. 
+    rewrite decide_spec. jauto. 
     (* is_closure *)
-    forwards Heq : pure_expr_pred_op1_lemma is_closure. eassumption. 
-    rewrite decide_spec. rewrite Heq. jauto. 
+    rewrite decide_spec. jauto. 
     (* is_object *)
-    forwards Heq : pure_expr_pred_op1_lemma is_object. eassumption. 
-    rewrite decide_spec. rewrite Heq. jauto. 
+    rewrite decide_spec. jauto. 
     (* prim_to_bool *)
-    forwards Heq : pure_expr_pred_op1_lemma value_to_bool_cast. eassumption. 
-    rewrite <- (isTrue_istrue (value_to_bool_cast v)).
-    rewrite Heq. jauto.
+    rew_refl. jauto.
     (* op2 *)
     forwards Hx : out_red_ter Hr2. reflexivity. destruct_hyp Hx.
     forwards Hpur : pure_expr_lemma Hr1. assumption. destruct_hyp Hpur. clear Hr1.
@@ -445,120 +400,147 @@ Proof.
     forwards Hx : out_red_ter Hr3. reflexivity. destruct_hyp Hx.
     forwards Hpur : pure_expr_lemma Hr2. assumption. destruct_hyp Hpur. clear Hr2.
     inverts Hr3 as Hr3; [idtac | false_abort].
-    destruct op; tryfalse; inverts Hr3 as Hr3; try false_invert.
+    destruct op; tryfalse; inverts keep Hr3 as Hr4; try false_invert.
     (* lt *)
-    inverts Hr3.
-    forwards Heq : pure_expr_pred_op2_number_lemma num_lt Hpur2 Hpur3.
-    rewrite <- (isTrue_istrue (num_lt n1 n2)).
-    rewrite Heq. jauto.
+    inverts keep Hr4.
+    rew_refl. jauto.
     (* le *)
-    inverts Hr3.
-    forwards Heq : pure_expr_pred_op2_number_lemma num_le Hpur2 Hpur3.
-    rewrite <- (isTrue_istrue (num_le n1 n2)).
-    rewrite Heq. jauto.
+    inverts keep Hr4.
+    rew_refl. jauto.
     (* gt *)
-    inverts Hr3.
-    forwards Heq : pure_expr_pred_op2_number_lemma num_gt Hpur2 Hpur3.
-    rewrite <- (isTrue_istrue (num_gt n1 n2)).
-    rewrite Heq. jauto.
+    inverts keep Hr4.
+    rew_refl. jauto.
     (* ge *)
-    inverts Hr3.
-    forwards Heq : pure_expr_pred_op2_number_lemma num_ge Hpur2 Hpur3.
-    rewrite <- (isTrue_istrue (num_ge n1 n2)).
-    rewrite Heq. jauto.
+    inverts keep Hr4.
+    rew_refl. jauto.
     (* stx_eq *) 
-    forwards Heq : pure_expr_pred_op2_lemma stx_eq Hpur2 Hpur3.
-    rewrite decide_spec. rewrite Heq. jauto.
+    rewrite decide_spec. jauto.
     (* same_value *)
-    forwards Heq : pure_expr_pred_op2_lemma same_value Hpur2 Hpur3.
-    rewrite decide_spec. rewrite Heq. jauto.
+    rewrite decide_spec. jauto.
     (* object_has_property *)
-    forwards Heq : pure_expr_pred_op2_object_string_lemma
-        (fun obj s => exists att, object_property_is st' obj s (Some att)) Hpur2 Hpur3 Hr3.
-    rewrite Heq. jauto.
+    rew_refl.
+    do 2 determine_epsilon. jauto.
     (* has_own_property *)
-    forwards Heq : pure_expr_pred_op2_object_string_lemma
-        (fun obj s => index (object_properties obj) s) Hpur2 Hpur3 Hr3.
-    rewrite decide_spec. rewrite Heq. jauto.
+    rew_refl. determine_epsilon. jauto.
     (* has_internal *)
-    forwards Heq : pure_expr_pred_op2_object_string_lemma
-        (fun obj s => index (object_internal obj) s) Hpur2 Hpur3 Hr3.
-    rewrite decide_spec. rewrite Heq. jauto.
+    rew_refl. determine_epsilon. jauto.
     (* is_accessor *)
-    forwards Heq : pure_expr_pred_op2_object_attrs_string_lemma
-        (fun obj s attrs => is_accessor attrs) Hpur2 Hpur3 Hr3. eassumption.
-    rewrite decide_spec. rewrite Heq. jauto.
+    rew_refl. do 2 determine_epsilon. jauto.
     (* string_lt *)
-    forwards Heq : pure_expr_pred_op2_string_lemma string_lt Hpur2 Hpur3.
-    rewrite <- (isTrue_istrue (string_lt s1 s2)).
-    rewrite Heq. jauto.
+    rew_refl. jauto.
     (* locale_compare *)
-    forwards Heq : pure_expr_pred_op2_string_lemma string_lt Hpur2 Hpur3.
-    rewrite <- (isTrue_istrue (string_lt s1 s2)).
-    rewrite Heq. jauto.
+    rew_refl. jauto.
+Qed.
+
+Lemma bool_red_expr_lemma_inv : forall c st e,
+    bool_expr e -> bool_expr_pre c st e -> 
+    red_expr c st e (out_ter st (res_value (value_bool (isTrue (bool_expr_pred c st e))))).
+Proof.
+    introv Hpe Hpre.
+    inductions Hpe gen c st Hpre; simpls; jauto.
+    (* bool *)
+    destruct b; rew_refl; eauto.
+    (* if *)
+    destruct Hpre as (Hpre1&Hpre2&Hpre3).
+    specializes IHHpe1 ___. eauto.
+    destruct (classic (bool_expr_pred c st e1));
+    [specializes IHHpe2 ___; eauto | specializes IHHpe3 ___; eauto];
+    rew_unreflect;
+    [rewrite isTrue_true in * by auto | rewrite isTrue_false in * by auto];
+    rew_bool;
+    eauto.
+    (* let *)
+    destruct_hyp Hpre.
+    forwards Hppre : pure_expr_lemma_inv. eassumption. eassumption.
+    jauto.
+    (* not *)
+    rew_refl. eauto. 
+    (* op1 *)
+    destruct op; tryfalse; destruct_hyp Hpre.
+    (* is_primitive *)
+    rewrite <- decide_spec. 
+    eauto using pure_expr_lemma_inv.
+    (* is_closure *)
+    rewrite <- decide_spec. 
+    eauto using pure_expr_lemma_inv.
+    (* is_object *)
+    rewrite <- decide_spec. 
+    eauto using pure_expr_lemma_inv.
+    (* prim_to_bool *)
+    rew_refl.
+    eauto using pure_expr_lemma_inv.
+    (* op2 *)
+    destruct op; tryfalse; 
+    destruct Hpre as (Hpre1&Hpre2&v&Heval);
+    inverts keep Heval as Hevalop; try inverts keep Hevalop. 
+    (* lt *)
+    rew_refl. eauto 80 using pure_expr_lemma_inv.
+    (* le *) 
+    rew_refl. eauto 80 using pure_expr_lemma_inv.
+    (* gt *)
+    rew_refl. eauto 80 using pure_expr_lemma_inv.
+    (* ge *) 
+    rew_refl. eauto 80 using pure_expr_lemma_inv.
+    (* stx_eq *)
+    rew_refl. rewrite <- decide_spec. 
+    eauto 8 using pure_expr_lemma_inv.
+    (* same_value *)
+    rew_refl. rewrite <- decide_spec. 
+    eauto 8 using pure_expr_lemma_inv.
+    (* has_property *)
+    rew_refl. do 2 determine_epsilon.
+    eauto 8 using pure_expr_lemma_inv.
+    (* has_own_property *)
+    determine_epsilon. rewrite <- decide_spec.
+    eauto 8 using pure_expr_lemma_inv.
+    (* has_internal *)
+    determine_epsilon. rewrite <- decide_spec.
+    eauto 8 using pure_expr_lemma_inv.
+    (* is_accessor *)
+    do 2 determine_epsilon. rewrite <- decide_spec.
+    eauto 8 using pure_expr_lemma_inv.
+    (* string_lt *)
+    rew_refl. eauto 80 using pure_expr_lemma_inv.
+    (* locale_compare *)
+    rew_refl. eauto 80 using pure_expr_lemma_inv.
 Qed.
 
 Module Export Tactics.
 
-Ltac object_property_is_determine_then :=
+Tactic Notation "object_property_is_determine" :=
     match goal with
     | H1 : object_property_is ?st ?obj ?name ?oattr1, H2 : object_property_is ?st ?obj ?name ?oattr2 |- _ =>
-        not constr_eq oattr1 oattr2; 
-        not is_hyp (oattr1 = oattr2);
-        let H := fresh "H" in asserts H : (oattr1 = oattr2); [eauto using object_property_is_deterministic | idtac];
-        revert H
+        not (first [constr_eq H1 H2 | constr_eq oattr1 oattr2 | is_hyp (oattr1=oattr2) | is_hyp (oattr2=oattr1)]);
+        determine H1 H2
     end.
 
-Ltac object_property_is_determine_eq := object_property_is_determine_then; intro.
-Ltac object_property_is_determine := object_property_is_determine_then; let H := fresh in intro H; try subst_hyp H.
-
-Ltac value_is_closure_determine_then :=
+Tactic Notation "value_is_closure_determine" :=
     match goal with
     | H1 : value_is_closure ?st ?v ?clo1, H2 : value_is_closure ?st ?v ?clo2 |- _ =>
-        not constr_eq clo1 clo2; 
-        not is_hyp (clo1 = clo2);
-        let H := fresh "H" in asserts H : (clo1 = clo2); [eauto using value_is_closure_deterministic | idtac];
-        revert H
+        not (first [constr_eq H1 H2 | constr_eq clo1 clo2 | is_hyp (clo1=clo2) | is_hyp (clo2=clo1)]);
+        determine H1 H2
     end.
 
-Ltac value_is_closure_determine_eq := value_is_closure_determine_then; intro.
-Ltac value_is_closure_determine := value_is_closure_determine_then; let H := fresh in intro H; try subst_hyp H.
-
-Ltac closure_ctx_determine_then :=
+Tactic Notation "closure_ctx_determine" :=
     match goal with
     | H1 : closure_ctx ?clo ?lv ?c1, H2 : closure_ctx ?clo ?lv ?c2 |- _ =>
-        not constr_eq c1 c2; 
-        not is_hyp (c1 = c2);
-        let H := fresh "H" in asserts H : (c1 = c2); [eauto using closure_ctx_deterministic | idtac];
-        revert H
+        not (first [constr_eq H1 H2 | constr_eq c1 c2 | is_hyp (c1=c2) | is_hyp (c2=c1)]);
+        determine H1 H2
     end.
 
-Ltac closure_ctx_determine_eq := closure_ctx_determine_then; intro.
-Ltac closure_ctx_determine := closure_ctx_determine_then; let H := fresh in intro H; try subst_hyp H.
-
-Ltac eval_unary_op_determine_then :=
+Tactic Notation "eval_unary_op_determine" :=
     match goal with
     | H1 : eval_unary_op ?op ?st ?v0 ?v1, H2 : eval_unary_op ?op ?st ?v0 ?v2 |- _ =>
-        not constr_eq v1 v2; 
-        not is_hyp (v1 = v2);
-        let H := fresh "H" in asserts H : (v1 = v2); [eauto using eval_unary_op_deterministic | idtac];
-        revert H
+        not (first [constr_eq H1 H2 | constr_eq v1 v2 | is_hyp (v1=v2) | is_hyp (v2=v1)]);
+        determine H1 H2
     end.
 
-Ltac eval_unary_op_determine_eq := eval_unary_op_determine_then; intro.
-Ltac eval_unary_op_determine := eval_unary_op_determine_then; let H := fresh in intro H; try subst_hyp H.
-
-Ltac eval_binary_op_determine_then :=
+Tactic Notation "eval_binary_op_determine" :=
     match goal with
     | H1 : eval_binary_op ?op ?st ?v0 ?v0' ?v1, H2 : eval_binary_op ?op ?st ?v0 ?v0' ?v2 |- _ =>
-        not constr_eq v1 v2; 
-        not is_hyp (v1 = v2);
-        let H := fresh "H" in asserts H : (v1 = v2); [eauto using eval_binary_op_deterministic | idtac];
-        revert H
+        not (first [constr_eq H1 H2 | constr_eq v1 v2 | is_hyp (v1=v2) | is_hyp (v2=v1)]);
+        determine H1 H2
     end.
-
-Ltac eval_binary_op_determine_eq := eval_binary_op_determine_then; intro.
-Ltac eval_binary_op_determine := eval_binary_op_determine_then; let H := fresh in intro H; try subst_hyp H.
 
 Ltac ljs_out_red_ter Hred :=
     let H := fresh in
@@ -577,6 +559,30 @@ Ltac ljs_bool_red_expr Hred :=
     lets H : bool_red_expr_lemma Hred; [solve [eauto 20 with ljs] | idtac];
     simpl in H; rew_logic in H; destruct_hyp H.
 
-Tactic Notation "ljs_bool_red_expr" "in" hyp(Hred) := ljs_bool_red_expr Hred; clear Hred.
+Tactic Notation "ljs_bool_red_expr" "in" hyp(Hred) := ljs_bool_red_expr Hred(*; clear Hred*).
+
+Ltac invert_binary_op :=
+    match goal with
+    | H : eval_binary_op _ _ _ _ _ |- _ =>
+        let H1 := fresh in
+        inverts H as H1; 
+        try match type of H1 with
+        | num_binary_op _ _ => inverts H1
+        | int_binary_op _ _ => inverts H1
+        | num_cmp_binary_op _ _ => inverts H1
+        end
+    end.
+
+Ltac invert_unary_op :=
+    match goal with
+    | H : eval_unary_op _ _ _ _ |- _ =>
+        let H1 := fresh in
+        inverts H as H1; 
+        try match type of H1 with
+        | num_unary_op _ _ => inverts H1
+        | int_unary_op _ _ => inverts H1
+        end
+    end.
 
 End Tactics.
+ 
