LambdaS5/coq/LibBagExt.v
@@ -120,9 +120,6 @@ Class Binds_double_eq `{BagBinds A B T} :=
 Class Binds_double `{BagBinds A B T} :=
     { binds_double : forall E F, (forall k x, binds E k x <-> binds F k x) -> E = F }.
 
-Class Binds_deterministic `{BagBinds A B T} :=
-    { binds_deterministic : forall E k x y, binds E k x -> binds E k y -> x = y }.
-
 (***** PROPERTIES RELATED TO BINDS *****)
 
 (* from_list *)
@@ -743,7 +740,7 @@ Proof. constructor. introv I. apply binds_double. intros. rewrite I. iauto. Qed.
 
 Global Instance Binds_deterministic_from_read_option_binds :
     forall `{BagBinds A B T} `{BagReadOption A B T},
-    Read_option_binds_eq -> Binds_deterministic.
+    Read_option_binds_eq -> forall m a, Deterministic (binds m a).
 Proof. 
     constructor. introv. rewrite_all <- read_option_binds_eq.
     introv Hx Hy.
@@ -1358,18 +1355,12 @@ Tactic Notation "rew_binds_eq" "~" "in" hyp(H) :=
 Tactic Notation "rew_binds_eq" "*" "in" hyp(H) :=
     rew_binds_eq in H; auto_star.
 
-Ltac binds_determine_then :=
+Tactic Notation "binds_determine" :=
     match goal with
     | H1 : binds ?m ?k ?v1, H2 : binds ?m ?k ?v2 |- _ =>
-        not constr_eq v1 v2; 
-        not is_hyp (v1 = v2);
-        let H := fresh "H" in asserts H : (v1 = v2); [eauto using binds_deterministic | idtac]; 
-        revert H2; revert H
+        not (first [constr_eq H1 H2 | constr_eq v1 v2 | is_hyp (v1 = v2) | is_hyp (v2 = v1)]);
+        determine H1 H2
     end.
-
-Ltac binds_determine_eq := binds_determine_then; intro; intro.
-Ltac binds_determine := binds_determine_then; 
-    let H := fresh "H" in let H1 := fresh "H" in intro H; intro H1; try (subst_hyp H; clear H1).
 
 Global Instance from_list_empty_from_from_list_binds_eq :
     forall `{BagFromList (A * B) T} `{BagEmpty T} `{BagBinds A B T},
